DynamoDbEncryption/runtimes/java/src/main/smithy-generated/software/amazon/cryptography/dbencryptionsdk/dynamodb/model/BeaconStyle.java
@@ -1,0 +1,192 @@
+// Copyright Amazon.com Inc. or its affiliates. All Rights Reserved.
+// SPDX-License-Identifier: Apache-2.0
+// Do not modify this file. This file is machine generated, and any changes to it will be overwritten.
+package software.amazon.cryptography.dbencryptionsdk.dynamodb.model;
+
+import java.util.Objects;
+
+public class BeaconStyle {
+  /**
+   * Attribute must be used as part of a Compound Beacon, never alone.
+   */
+  private final PartOnly partOnly;
+
+  /**
+   * This beacon should calculate values like another beacon, so they can be compared.
+   */
+  private final Twinned twinned;
+
+  /**
+   * Attribute must be a Set. Beacon value will also be a Set.
+   */
+  private final AsSet asSet;
+
+  /**
+   * Both Twinned and AsSet.
+   */
+  private final TwinnedSet twinnedSet;
+
+  protected BeaconStyle(BuilderImpl builder) {
+    this.partOnly = builder.partOnly();
+    this.twinned = builder.twinned();
+    this.asSet = builder.asSet();
+    this.twinnedSet = builder.twinnedSet();
+  }
+
+  /**
+   * @return Attribute must be used as part of a Compound Beacon, never alone.
+   */
+  public PartOnly partOnly() {
+    return this.partOnly;
+  }
+
+  /**
+   * @return This beacon should calculate values like another beacon, so they can be compared.
+   */
+  public Twinned twinned() {
+    return this.twinned;
+  }
+
+  /**
+   * @return Attribute must be a Set. Beacon value will also be a Set.
+   */
+  public AsSet asSet() {
+    return this.asSet;
+  }
+
+  /**
+   * @return Both Twinned and AsSet.
+   */
+  public TwinnedSet twinnedSet() {
+    return this.twinnedSet;
+  }
+
+  public Builder toBuilder() {
+    return new BuilderImpl(this);
+  }
+
+  public static Builder builder() {
+    return new BuilderImpl();
+  }
+
+  public interface Builder {
+    /**
+     * @param partOnly Attribute must be used as part of a Compound Beacon, never alone.
+     */
+    Builder partOnly(PartOnly partOnly);
+
+    /**
+     * @return Attribute must be used as part of a Compound Beacon, never alone.
+     */
+    PartOnly partOnly();
+
+    /**
+     * @param twinned This beacon should calculate values like another beacon, so they can be compared.
+     */
+    Builder twinned(Twinned twinned);
+
+    /**
+     * @return This beacon should calculate values like another beacon, so they can be compared.
+     */
+    Twinned twinned();
+
+    /**
+     * @param asSet Attribute must be a Set. Beacon value will also be a Set.
+     */
+    Builder asSet(AsSet asSet);
+
+    /**
+     * @return Attribute must be a Set. Beacon value will also be a Set.
+     */
+    AsSet asSet();
+
+    /**
+     * @param twinnedSet Both Twinned and AsSet.
+     */
+    Builder twinnedSet(TwinnedSet twinnedSet);
+
+    /**
+     * @return Both Twinned and AsSet.
+     */
+    TwinnedSet twinnedSet();
+
+    BeaconStyle build();
+  }
+
+  static class BuilderImpl implements Builder {
+    protected PartOnly partOnly;
+
+    protected Twinned twinned;
+
+    protected AsSet asSet;
+
+    protected TwinnedSet twinnedSet;
+
+    protected BuilderImpl() {
+    }
+
+    protected BuilderImpl(BeaconStyle model) {
+      this.partOnly = model.partOnly();
+      this.twinned = model.twinned();
+      this.asSet = model.asSet();
+      this.twinnedSet = model.twinnedSet();
+    }
+
+    public Builder partOnly(PartOnly partOnly) {
+      this.partOnly = partOnly;
+      return this;
+    }
+
+    public PartOnly partOnly() {
+      return this.partOnly;
+    }
+
+    public Builder twinned(Twinned twinned) {
+      this.twinned = twinned;
+      return this;
+    }
+
+    public Twinned twinned() {
+      return this.twinned;
+    }
+
+    public Builder asSet(AsSet asSet) {
+      this.asSet = asSet;
+      return this;
+    }
+
+    public AsSet asSet() {
+      return this.asSet;
+    }
+
+    public Builder twinnedSet(TwinnedSet twinnedSet) {
+      this.twinnedSet = twinnedSet;
+      return this;
+    }
+
+    public TwinnedSet twinnedSet() {
+      return this.twinnedSet;
+    }
+
+    public BeaconStyle build() {
+      if (!onlyOneNonNull()) {
+        throw new IllegalArgumentException("`BeaconStyle` is a Union. A Union MUST have one and only one value set.");
+      }
+      return new BeaconStyle(this);
+    }
+
+    private boolean onlyOneNonNull() {
+      Object[] allValues = {this.partOnly, this.twinned, this.asSet, this.twinnedSet};
+      boolean haveOneNonNull = false;
+      for (Object o : allValues) {
+        if (Objects.nonNull(o)) {
+          if (haveOneNonNull) {
+            return false;
+          }
+          haveOneNonNull = true;
+        }
+      }
+      return haveOneNonNull;
+    }
+  }
+}
