DynamoDbEncryption/dafny/DynamoDbEncryption/src/SearchInfo.dfy
@@ -384,7 +384,7 @@ module SearchableEncryptionInfo {
         cmp.isEncrypted()
     }
     function method hash(item : DDB.AttributeMap, vf : VirtualFieldMap, keys : MaybeKeyMap)
-      : (ret : Result<Option<string>, Error>)
+      : (ret : Result<Option<DDB.AttributeValue>, Error>)
       requires !keys.DontUseKeys?
 
       //= specification/searchable-encryption/search-config.md#get-beacon-key-for-query
@@ -394,13 +394,17 @@ module SearchableEncryptionInfo {
       ensures Standard? && keys.ShouldHaveKeys? ==> ret.Failure?
     {
       if Standard? then
-        :- Need(keys.Keys?, E("Need key for beacon " + std.base.name + " but no keyId found in query."));
-        if std.base.name in keys.value then
-          std.getHash(item, vf, keys.value[std.base.name])
+        :- Need(keys.Keys?, E("Need key for beacon " + std.keyName() + " but no keyId found in query."));
+        if std.keyName() in keys.value then
+          std.getHash(item, vf, keys.value[std.keyName()])
         else
-          Failure(E("Internal error. Beacon " + std.base.name + " has no key."))
+          Failure(E("Internal error. Beacon " + std.keyName() + " has no key!"))
       else
-        cmp.hash(item, vf, keys)
+        var strHash :- cmp.hash(item, vf, keys);
+        if strHash.None? then
+          Success(None)
+        else
+          Success(Some(DDB.AttributeValue.S(strHash.value)))
     }
     function method naked(item : DDB.AttributeMap, vf : VirtualFieldMap) : Result<Option<DDB.AttributeValue>, Error>
     {
@@ -418,11 +422,7 @@ module SearchableEncryptionInfo {
       if keys.DontUseKeys? then
         naked(item, vf)
       else
-        var str :- hash(item, vf, keys);
-        if str.None? then
-          Success(None)
-        else
-          Success(Some(DS(str.value)))
+        hash(item, vf, keys)
     }
     function method getName() : string
     {
@@ -446,17 +446,18 @@ module SearchableEncryptionInfo {
         cmp.GetFields(virtualFields)
     }
 
-    function method GetBeaconValue(value : DDB.AttributeValue, keys : MaybeKeyMap, forEquality : bool) : Result<DDB.AttributeValue, Error>
+    function method GetBeaconValue(value : DDB.AttributeValue, keys : MaybeKeyMap, forEquality : bool)
+      : Result<DDB.AttributeValue, Error>
     {
       if keys.DontUseKeys? then
         Success(value)
       else if Standard? then
-        :- Need(!keys.ShouldHaveKeys?, E("Need KeyId because of beacon " + std.base.name + " but no KeyId found in query"));
+        :- Need(!keys.ShouldHaveKeys?, E("Need KeyId because of beacon " + std.keyName() + " but no KeyId found in query"));
         var keys := keys.value;
-        if std.base.name in keys then
-          std.GetBeaconValue(value, keys[std.base.name])
+        if std.keyName() in keys then
+          std.GetBeaconValue(value, keys[std.keyName()])
         else
-          Failure(E("Internal error. Beacon " + std.base.name + " has no key."))
+          Failure(E("Internal error. Beacon " + std.keyName() + " has no key."))
       else
         cmp.GetBeaconValue(value, keys, forEquality)
     }
@@ -482,6 +483,10 @@ module SearchableEncryptionInfo {
     | SignedBeacon
     | EncryptedBeacon
 
+  predicate method IsPartOnly(b : Beacon)
+  {
+    b.Standard? && b.std.partOnly
+  }
   predicate method IsBeaconOfType(b : Beacon, t : BeaconType)
   {
     match t {
@@ -718,7 +723,9 @@ module SearchableEncryptionInfo {
     {
       if |names| == 0 then
         Success(acc)
-      else if IsBeaconOfType(beacons[names[0]], bType) then
+      //= specification/searchable-encryption/beacons.md#partonly-initialization
+      //# The Standard Beacon MUST NOT be stored in the item for a PartOnly beacon.
+      else if IsBeaconOfType(beacons[names[0]], bType) && !IsPartOnly(beacons[names[0]]) then
         var value :- GenerateBeacon(names[0], item, keys);
         if value.Some? then
           GenerateBeacons2(names[1..], item, keys, bType, acc[beacons[names[0]].getBeaconName() := value.value])
